proofs/Symcrust/Properties.lean
@@ -2,3 +2,260 @@ import Symcrust.Arith
 import Symcrust.BarrettReduction
 import Symcrust.MontReduction
 import Symcrust.SpecAux
+import Symcrust.NatBit
+
+import Symcrust.Funs
+
+open Aeneas
+open Std
+open Result
+
+namespace Symcrust -- TODO: fix namespace issues
+
+def ntt.SymCryptMlKemModAdd' (a : U32) (b : U32) : Result U32 :=
+  do
+  massert (a < ntt.Q)
+  massert (b < ntt.Q)
+  let i ← a + b
+  let res := core.num.U32.wrapping_sub i ntt.Q
+  let i1 ← res >>> 16#i32
+  (if i1 = 0#u32 then ok () else massert (i1 = 65535#u32))
+  let res1 := core.num.U32.wrapping_add res (ntt.Q &&& i1)
+  massert (res1 < ntt.Q)
+  Result.ok res1
+
+-- TODO: move
+@[simp]
+def bind_eq_iff (x : Result α) (y y' : α → Result β) :
+  ((Bind.bind x y) = (Bind.bind x y')) ↔
+  ∀ v, x = ok v → y v = y' v := by
+  dcases x <;> simp_all
+
+@[simp]
+def ntt.SymCryptMlKemModAdd_eq (a : U32) (b : U32) :
+  SymCryptMlKemModAdd a b = SymCryptMlKemModAdd' a b := by
+  unfold SymCryptMlKemModAdd SymCryptMlKemModAdd'
+  simp
+  intros
+  split <;> simp
+
+@[simp]
+theorem ntt.Q_eq : Q = 3329#u32 := by
+  unfold Q Q_body eval_global
+  simp
+
+attribute [local simp] Spec.Q -- TODO: add this to the scalar_tac simp set
+
+-- TODO: move
+@[pspec]
+theorem massert_spec (b : Bool) (h : b) :
+  massert b = ok () := by
+  simp [massert, *]
+
+-- TODO: move
+@[pspec]
+theorem massert_decide_spec (b : Prop) [Decidable b] (h : b) :
+  massert (decide b) = ok () := by
+  simp [massert, *]
+
+-- TODO: generalize, move
+@[simp] theorem core.num.U32.and_val (x y : U32) :
+  (x &&& y).val = Int.land x.val y.val := by
+  sorry
+
+-- TODO: move
+theorem Int.eq_of_testBit_eq {x y : Int}
+  (pred : ∀ (i : ℕ), x.testBit i = y.testBit i) : x = y := by
+  cases x <;> cases y <;> rename_i x y <;> simp only [Int.testBit] at pred
+  . have : x = y := by
+      apply Nat.eq_of_testBit_eq
+      apply pred
+    rw [this]
+  . -- Contradiction
+    sorry
+  . -- Contradiction
+    sorry
+  . have : x = y := by
+      apply Nat.eq_of_testBit_eq
+      intro i
+      replace pred := pred i
+      simp at pred
+      apply pred
+    rw [this]
+
+@[simp]
+theorem Int.testBit_zero (i : Nat) : Int.testBit 0 i = false := by
+  unfold Int.testBit; simp
+
+-- TODO: move
+@[simp] theorem Int.land_zero_right (x : Int) :
+  Int.land x 0 = 0 := by
+  apply Int.eq_of_testBit_eq
+  intro i
+  simp
+
+-- TODO: move
+@[simp] theorem Int.land_zero_left (x : Int) :
+  Int.land 0 x = 0 := by
+  apply Int.eq_of_testBit_eq
+  intro i
+  simp
+
+@[simp]
+theorem Int.testBit_pos_eq_nat_testBit (x i : Nat) :
+  (x : Int).testBit i = x.testBit i := by
+  unfold Int.testBit; simp
+
+example (x : BitVec 32) (h : x ≤ BitVec.ofInt 32 (2^4)) :
+  x >>> 5 = 0 := by
+  bv_decide
+
+#eval (BitVec.ofNat 32 (2^32-1)) >>> 31
+#eval (BitVec.ofInt 32 (2^32))
+#eval (BitVec.ofNat 32 (2^32-1)) &&& 0
+#check Int.bmod
+
+example (n m : BitVec 32) (hn : n < BitVec.ofInt 32 (2 ^ 16)) (hm : m < BitVec.ofInt 32 (2 ^ 16)) :
+  m &&& ((BitVec.ofNat 32 (2^32 - 1) - n) >>> 16) = m := by
+  bv_decide
+
+theorem Int.testBit_two_pow_sub_succ {x : Int} {n : ℕ} (h₁ : 0 ≤ x) (h₂ : x < 2 ^ n) (i : ℕ) :
+  (2 ^ n - (x + 1)).testBit i = (i < n && !x.testBit i) := by
+  have hx : x = x.toNat := by omega
+  have h1 := @Nat.testBit_two_pow_sub_succ x.toNat n (by norm_cast at *; omega) i
+  simp at *
+  have h2 := Int.testBit_pos_eq_nat_testBit (2 ^ n - (x + 1).toNat) i
+  have : (2^n - (x + 1).toNat : Nat) = 2 ^n - (x + 1) := by
+    norm_cast at *
+    omega
+  rw [this] at h2; clear this
+  rw [h2]; clear h2
+
+  have : 2 ^ n - (x.toNat + 1) = 2 ^ n - (x + 1).toNat := by
+    norm_cast at *
+    omega
+  rw [this] at h1; clear this
+  rw [h1]; clear h1
+
+  have : x.toNat.testBit i = x.testBit i := by
+    sorry
+  simp [this]
+
+#check Nat.testBit_shiftRight
+
+@[simp] theorem Int.testBit_shiftRight {i j : Nat} (x : Int) :
+  (x >>> i).testBit j = x.testBit (i + j) := by
+  sorry
+
+@[simp] theorem Int.testBit_int_shiftRight {i : Int} {j : Nat} (x : Int) :
+  (x >>> i).testBit j = x.testBit (i.toNat + j) := by
+  sorry
+
+/-theorem Int.testBit_shiftLeft {i j : Nat}  (x : Int) :
+  (x <<< i).testBit j = (j ≥ i && x.testBit (j - i)) := by sorry-/
+
+#check Nat.testBit_eq_false_of_lt
+
+theorem Int.testBit_pos_eq_false_of_lt {n : Int} {i : ℕ} (h : 0 ≤ n) (h : n < 2 ^ i) :
+  n.testBit i = false := by
+  sorry
+
+-- TODO: move
+theorem ntt.SymCryptMlKemMod_underflow_eq
+  (n m : Int) (hn0 : 0 ≤ n) (hn : n < 2 ^ 12) (hm0 : 0 ≤ m) (hm : m < 2 ^ 12):
+  Int.land m ((2^32 - 1 - n) >>> (16 : Nat)) = m := by
+  apply Int.eq_of_testBit_eq
+  intro i
+  have h : 2^32 - 1 - n = 2^32 - (n + 1) := by ring_nf
+  rw [h]; clear h
+  have := @Int.testBit_two_pow_sub_succ n 32 (by omega) (by omega) (16 + i)
+  simp [-Int.reducePow]
+  rw [this]; clear this
+  intro hi
+  dcases hi : i < 12
+  . simp; split_conjs
+    . omega
+    . have hi : n < 2^(16 + i) := by
+        have := @Int.pow_le_pow_of_le_right 2 (by simp) 12 (16 + i) (by omega)
+        norm_cast at *
+        omega
+      apply @Int.testBit_pos_eq_false_of_lt n (16 + i) (by omega) hi
+  . -- Contradiction
+    have hi : m < 2^i := by
+      have := @Int.pow_le_pow_of_le_right 2 (by simp) 12 i (by omega)
+      norm_cast at *
+      omega
+    have := @Int.testBit_pos_eq_false_of_lt m i (by omega) hi
+    simp_all
+
+theorem ntt.SymCryptMlKemMod'_spec (a : U32) (b : U32)
+  (ha : a.val < Spec.Q) (hb : b.val < Spec.Q) :
+  ∃ (c : U32), ntt.SymCryptMlKemModAdd' a b = ok c ∧
+  (c.val : Spec.Zq) = (a.val : Spec.Zq) + (b.val : Spec.Zq) ∧
+  c.val < Spec.Q := by
+  unfold SymCryptMlKemModAdd'
+  simp at *
+  progress
+  progress
+  progress as ⟨ c1, hc1 ⟩
+  progress as ⟨ c2, hc2 ⟩
+  simp at *
+  -- TODO: handle this properly with progress
+  have hIf : (if c2 = 0#u32 then ok () else massert (c2 = 65535#u32)) = ok () := by
+    split <;> simp_all
+    sorry
+  progress; clear hIf
+  --
+  progress
+  . sorry -- This is the assert
+  . simp
+    -- There are two cases depending on whether `a + b - q` is `< 0` or not
+    dcases hlt : 0 ≤ a.val + b.val - 3329
+    . -- No underflow
+      let c : Int := a.val + b.val - 3329
+      have : 0 ≤ c ∧ c < 3329 := by scalar_tac
+      have hcMod : c % (U32.max + 1) = c := by
+        apply Int.emod_eq_of_lt <;> scalar_tac
+      have hc2Eq : c2.val = 0 := by
+        rw [hc2, hc1, hcMod]
+        rw [Int.shiftRight_eq_div_pow]
+        apply Int.ediv_eq_zero_of_lt <;>
+        scalar_tac
+      rw [hc2Eq]
+      simp [*]
+      rw [hcMod]
+      simp +zetaDelta [Spec.Zq]
+      split_conjs
+      . rfl
+      . scalar_tac
+    . -- Underflow
+      simp at hlt
+      have hAnd : Int.land 3329 c2.val = 3329 := by
+        -- This is the tricky proof
+        have hc1Mod :=
+          calc
+            (c1.val - 3329) % (U32.max + 1) =
+              (U32.max + 1 - (3329 - c1.val)) % (U32.max + 1) := by
+              have := @Int.add_emod_self_left (U32.max + 1) (c1.val - 3329)
+              rw [← this]
+              ring_nf
+            _ = U32.max + 1 - (3329 - c1.val) := by
+              apply Int.emod_eq_of_lt <;> scalar_tac
+
+        rw [hc2, hc1Mod]
+        have hEq := ntt.SymCryptMlKemMod_underflow_eq (3329 - c1.val - 1) 3329 (by scalar_tac) (by scalar_tac) (by simp) (by simp)
+        ring_nf at hEq
+        simp [U32.max]
+        ring_nf
+        apply hEq
+      rw [hAnd]
+      simp
+
+      have hMod : c1.val % (U32.max + 1) = c1.val := by
+        apply Int.emod_eq_of_lt <;> scalar_tac
+      rw [hMod]
+      split_conjs
+      . simp [*]
+      . scalar_tac
+
+end Symcrust
